theories/type_systems/stlc_extended_sol/lang.v
@@ -137,6 +137,50 @@ Proof.
   apply is_val_spec. rewrite to_of_val. by eexists.
 Qed.
 
+(** Now we are finally ready to define the actual big-step evaluation relation. *)
+
+Inductive big_step : expr -> val -> Prop :=
+  | BsLitInt (n : Z) :
+      big_step (LitInt n) (LitIntV n)
+  | BsLam (x : string) (e : expr) :
+      big_step (Lam x e) (LamV x e)
+  | BsPlus e1 e2 (z1 z2 : Z) :
+      big_step e1 (LitIntV z1) ->
+      big_step e2 (LitIntV z2) ->
+      big_step (Plus e1 e2) (LitIntV (z1 + z2))%Z
+  | BisApp e1 e2 x e v2 v :
+      big_step e1 (@LamV x e) ->
+      big_step e2 v2 ->
+      big_step (subst x (of_val v2) e) v ->
+      big_step (App e1 e2) v
+  | BsPair e1 e2 (v w : val) :
+      big_step e1 v ->
+      big_step e2 w ->
+      big_step (Pair e1 e2) (PairV v w)
+  | BsProj1 e v w :
+      big_step e (PairV v w) ->
+      big_step (Proj1 e) v
+  | BsProj2 e v w :
+      big_step e (PairV v w) ->
+      big_step (Proj2 e) w
+.
+#[export] Hint Constructors big_step : core.
+
+(** We can show that values behave the way they should. *)
+Lemma big_step_vals (v : val) : big_step (of_val v) v.
+Proof.
+  induction v; try constructor; done.
+Qed.
+
+Lemma big_step_inv_vals (v w : val) : big_step (of_val v) w -> v = w.
+Proof.
+  (** [inversion 1] means "do inversion on the first assumption in the goal",
+  i.e., it is the same as [intros H; inversion H]. *)
+  revert w.
+  induction v; inversion 1; try reflexivity.
+  simplify_eq. apply IHv2 in H4 as ->. apply IHv1 in H2 as ->. reflexivity.
+Qed.
+
 (** *** Contextual Semantics *)
 (** Base reduction *)
 Inductive base_step : expr -> expr -> Prop :=
