theories/type_systems/stlc_extended/closed.v
@@ -1,0 +1,52 @@
+From ffpl.lib Require Import prelude sets.
+From ffpl.type_systems.stlc_extended Require Export lang.
+
+(** Open and closed expressions.
+In the lecture notes we formalize the "set of free variables" of a term.
+For Coq it turns out to be sufficient, and easier, to instead define a predicate
+that says whether a set [X] contains all free variables:
+[is_closed X e] evaluates to [true] iff all free variables in [e] are contained in [X].
+We define this as a functon that returns a [bool], i.e. this actually computes an
+answer that is either [true] or [false]. *)
+Fixpoint is_closed (X : gset string) (e : expr) : bool :=
+  match e with
+  | Var x => bool_decide (x `elem` X)
+  | Lam x e => is_closed ({[x]} `union` X) e
+  | LitInt _ => true
+  | App e1 e2
+  | Plus e1 e2 => is_closed X e1 && is_closed X e2
+  | Pair e1 e2 => is_closed X e1 && is_closed X e2
+  | Proj1 e => is_closed X e
+  | Proj2 e => is_closed X e
+  end.
+
+(** We can compute with this definition. *)
+Compute (is_closed empty (LitInt 0)).
+Compute (is_closed empty (Var "x")).
+Compute (is_closed {["x"]} (Var "x")).
+
+(** [closed X e] is the propositional version of [is_closed X e]:
+[closed X e] has type [Prop], not [bool]. *)
+Notation closed X e := (Is_true (is_closed X e)).
+
+(** Defining it like this means we can do proofs "by computation". *)
+Example lit_is_closed z : closed empty (LitInt z).
+Proof. simpl. done. Qed.
+
+(** We show some key properties of [closed].
+We don't expect you to be able to do these proofs ([Is_true] can be
+somewhat tricky to work with); we will provide all the results you need. *)
+Lemma closed_weaken X Y e : closed X e -> subseteq X Y -> closed Y e.
+Proof. revert X Y; induction e; naive_solver (eauto; set_solver). Qed.
+
+Lemma closed_weaken_nil X e : closed empty e -> closed X e.
+Proof. intros. by apply closed_weaken with empty, empty_subseteq. Qed.
+
+Lemma subst_closed X e x es : closed X e -> ~(x `elem` X) -> subst x es e = e.
+Proof.
+  induction e in X |- *; simpl; rewrite ?bool_decide_spec ?andb_True; intros ??;
+    repeat case_decide; simplify_eq; simpl; f_equal; intuition eauto with set_solver.
+Qed.
+
+Lemma subst_closed_nil e x es : closed empty e -> subst x es e = e.
+Proof. intros. apply subst_closed with empty; done || set_solver. Qed.
