theories/type_systems/stlc_extended_sol/parallel_subst.v
@@ -1,0 +1,95 @@
+From stdpp Require Import prelude.
+From ffpl.lib Require Import prelude.
+From ffpl.lib Require Export maps.
+From ffpl.type_systems.stlc_extended_sol Require Import lang notation closed.
+
+(** * Parallel substitution *)
+
+(** This is the parallel substitution operation. We represent a substitution map
+as a finite map [xs]. We use maps of [expr] to be able to reuse [closed]. *)
+Fixpoint subst_map (xs : gmap string expr) (e : expr) : expr :=
+  match e with
+  | LitInt n => LitInt n
+  | Var y => match xs !! y with Some es => es | _ =>  Var y end
+  | App e1 e2 => App (subst_map xs e1) (subst_map xs e2)
+  | Lam x e => Lam x (subst_map (delete x xs) e)
+  | Plus e1 e2 => Plus (subst_map xs e1) (subst_map xs e2)
+  | Pair e1 e2 => Pair (subst_map xs e1) (subst_map xs e2)
+  | Proj1 e => Proj1 (subst_map xs e)
+  | Proj2 e => Proj2 (subst_map xs e)
+  end.
+
+(** We lift the notion of closedness [closed] to substitution maps. *)
+Definition subst_closed (X : gset string) (map : gmap string expr) :=
+  forall x e, map !! x = Some e -> closed X e.
+
+(** Some lemmas about these definitions. We don't expect you to be able to do
+these proofs; we will provide all the results you need. *)
+
+Lemma subst_map_empty e :
+  subst_map empty e = e.
+Proof.
+  induction e; simpl; f_equal; [|by eauto..].
+  by rewrite !delete_empty.
+Qed.
+
+Lemma subst_closed_weaken X Y map1 map2 :
+  Y `subseteq` X -> map1 `subseteq` map2 -> subst_closed Y map2 -> subst_closed X map1.
+Proof.
+  intros Hsub1 Hsub2 Hclosed2 x e Hl.
+  eapply closed_weaken. 1:eapply Hclosed2, map_subseteq_spec; done. done.
+Qed.
+
+(** Lemma about the interaction with "normal" substitution. *)
+Lemma subst_subst_map x es gamma e :
+  subst_closed empty gamma ->
+  subst x es (subst_map (delete x gamma) e) =
+  subst_map (<[x:=es]> gamma) e.
+Proof.
+  revert gamma es x; induction e; intros gamma v0 xx Hclosed; simpl;
+  try (f_equal; eauto).
+  - destruct (decide (xx=x)) as [->|Hne].
+    + rewrite lookup_delete_eq // lookup_insert_eq //. simpl.
+      rewrite decide_True //.
+    + rewrite lookup_delete_ne // lookup_insert_ne //.
+      destruct (_ !! x) as [rr|] eqn:Helem.
+      * apply Hclosed in Helem.
+        by apply subst_closed_nil.
+      * simpl. rewrite decide_False //.
+  - case_decide.
+    + simplify_eq. rewrite delete_idemp delete_insert_delete. done.
+    + rewrite delete_insert_ne //. rewrite delete_commute. apply IHe.
+      eapply subst_closed_weaken; [done| |done].
+      apply map_delete_subseteq.
+Qed.
+
+(** Lemma about when the result of [subst_map] is closed:
+for [subst_map gamma e] to be closed under X, we need [gamma] itself to be
+closed under [X], and [e] to be closed under [X] plus everything defined in
+[gamma]. In other words, [subst_map gamma] removes [dom gamma] from the set of
+free variables of [e], if [gamma] is itself sufficiently closed. *)
+Lemma closed_subst_map X gamma e:
+  closed (X `union` dom gamma) e ->
+  subst_closed X gamma ->
+  closed X (subst_map gamma e).
+Proof.
+  induction e in X, gamma |-*; simpl.
+  - intros Hel%bool_decide_unpack Hcl.
+    destruct (gamma !! x) eqn:EQ.
+    + by eapply Hcl.
+    + simpl. apply bool_decide_pack.
+      apply not_elem_of_dom in EQ. set_solver.
+  - intros Hcl Hcl'.
+    eapply IHe.
+    2:{ eapply subst_closed_weaken; last done. 1:set_solver.
+        apply map_delete_subseteq. }
+    eapply closed_weaken; first done.
+    rewrite dom_delete.
+    intros y. destruct (decide (x = y)); set_solver.
+  - rewrite !andb_True. intros [H1 H2] Hcl. split; eauto.
+  - auto.
+  - rewrite !andb_True. intros [H1 H2] Hcl. split; eauto.
+  - rewrite !andb_True. intros [H1 H2] Hcl. split; eauto.
+  - eauto.
+  - eauto.
+Qed.
